src/project.rs
@@ -16,6 +16,8 @@ const PROJECT_REVISION_SCHEMA: &str = "fr-project-revision-4";
 
 pub mod author;
 pub use author::{disclosed_edit_admitted, disclosed_ir_edit_admitted};
+pub(crate) mod agent_intent;
+pub use agent_intent::agent_intent_section_allowed;
 mod batch;
 mod components;
 mod configuration;
